examples/conn/proofs/base.v
@@ -13,7 +13,7 @@ Set Implicit Arguments.
 Unset Strict Implicit.
 Unset Printing Implicit Defensive.
 
-Notation connN := (nroot.@"conn").
+Local Notation connN := (nroot.@"conn").
 
 Record state := State {
   cs_si   :> sess_info;
