examples/store/proofs/server/store.v
@@ -15,7 +15,7 @@ Unset Printing Implicit Defensive.
 
 Section Verif.
 
-Context `{!cryptisGS Σ, !heapGS Σ, !Conn.connGS Σ, !RPC.rpcGS Σ}.
+Context `{!cryptisGS Σ, !heapGS Σ, !iso_dhGS Σ, !Conn.connGS Σ, !RPC.rpcGS Σ}.
 Notation iProp := (iProp Σ).
 
 Context `{!storeGS Σ}.
